binders based on handshake messages

src/tls/ParsersAux.Binders.fsti
@@ -7,20 +7,28 @@ module U32 = FStar.UInt32
 (* ClientHello binders *)
 
 module L = FStar.List.Tot
+module H = Parsers.Handshake
 module CH = Parsers.ClientHello
 module CHE = Parsers.ClientHelloExtension
 
-let has_binders (c: CH.clientHello) : Tot Type0 = (* TODO: harmonize with HSL.Transcript.client_hello_has_psk *)
-  Cons? (c.CH.extensions) /\
+let has_binders (m: H.handshake) : Tot bool = (* TODO: harmonize with HSL.Transcript.client_hello_has_psk *)
+  H.M_client_hello? m && (
+  let c = H.M_client_hello?._0 m in
+  Cons? (c.CH.extensions) &&
   CHE.CHE_pre_shared_key? (L.last c.CH.extensions)
+  )
 
 module Psks = Parsers.OfferedPsks
 
-let get_binders (c: CH.clientHello {has_binders c}) : Tot Psks.offeredPsks_binders =
+let get_binders (m: H.handshake {has_binders m}) : Tot Psks.offeredPsks_binders =
+  let c = H.M_client_hello?._0 m in
   (CHE.CHE_pre_shared_key?._0 (L.last c.CH.extensions)).Psks.binders
 
-val set_binders (c: CH.clientHello {has_binders c}) (b' : Psks.offeredPsks_binders { Psks.offeredPsks_binders_bytesize b' == Psks.offeredPsks_binders_bytesize (get_binders c)})
-  : GTot (c' : CH.clientHello {
+val set_binders (m: H.handshake {has_binders m}) (b' : Psks.offeredPsks_binders { Psks.offeredPsks_binders_bytesize b' == Psks.offeredPsks_binders_bytesize (get_binders m)})
+  : Tot (m' : H.handshake {
+    has_binders m' /\ (
+    let c = H.M_client_hello?._0 m in
+    let c' = H.M_client_hello?._0 m' in
     c'.CH.version == c.CH.version /\
     c'.CH.random == c.CH.random /\
     c'.CH.session_id == c.CH.session_id /\
@@ -30,8 +38,8 @@ val set_binders (c: CH.clientHello {has_binders c}) (b' : Psks.offeredPsks_binde
     L.init c'.CH.extensions == L.init c.CH.extensions /\
     CHE.CHE_pre_shared_key? (L.last c'.CH.extensions) /\
     (CHE.CHE_pre_shared_key?._0 (L.last c'.CH.extensions)).Psks.identities == (CHE.CHE_pre_shared_key?._0 (L.last c.CH.extensions)).Psks.identities /\
-    get_binders c' == b'
-  })
+    get_binders m' == b'
+  )})
 
 let rec list_append_init_last (#a: Type) (l: list a { Cons? l }) : Lemma
   (l == L.append (L.init l) [L.last l])
@@ -56,88 +64,88 @@ let list_init_last_inj (#a: Type) (l1: list a { Cons? l1 } ) (l2: list a { Cons?
 = list_append_init_last l1;
   list_append_init_last l2
 
-let set_binders_get_binders (c: CH.clientHello {has_binders c}) : Lemma
-  (set_binders c (get_binders c) == c)
-= list_init_last_inj c.CH.extensions (set_binders c (get_binders c)).CH.extensions
+let set_binders_get_binders (m: H.handshake {has_binders m}) : Lemma
+  (set_binders m (get_binders m) == m)
+= list_init_last_inj (H.M_client_hello?._0 m).CH.extensions (H.M_client_hello?._0 (set_binders m (get_binders m))).CH.extensions
 
 val set_binders_bytesize
-  (c: CH.clientHello {has_binders c})
-  (b' : Psks.offeredPsks_binders { Psks.offeredPsks_binders_bytesize b' == Psks.offeredPsks_binders_bytesize (get_binders c)})
+  (m: H.handshake {has_binders m})
+  (b' : Psks.offeredPsks_binders { Psks.offeredPsks_binders_bytesize b' == Psks.offeredPsks_binders_bytesize (get_binders m)})
 : Lemma
-  (CH.clientHello_bytesize (set_binders c b') == CH.clientHello_bytesize c)
+  (H.handshake_bytesize (set_binders m b') == H.handshake_bytesize m)
 
 let set_binders_set_binders
-  (c: CH.clientHello {has_binders c})
-  (b1: Psks.offeredPsks_binders { Psks.offeredPsks_binders_bytesize b1 == Psks.offeredPsks_binders_bytesize (get_binders c)})
+  (m: H.handshake {has_binders m})
+  (b1: Psks.offeredPsks_binders { Psks.offeredPsks_binders_bytesize b1 == Psks.offeredPsks_binders_bytesize (get_binders m)})
   (b2: Psks.offeredPsks_binders { Psks.offeredPsks_binders_bytesize b2 == Psks.offeredPsks_binders_bytesize b1})
 : Lemma
-  (set_binders (set_binders c b1) b2 == set_binders c b2)
-= list_init_last_inj (set_binders (set_binders c b1) b2).CH.extensions (set_binders c b2).CH.extensions
+  (set_binders (set_binders m b1) b2 == set_binders m b2)
+= list_init_last_inj (H.M_client_hello?._0 (set_binders (set_binders m b1) b2)).CH.extensions (H.M_client_hello?._0 (set_binders m b2)).CH.extensions
 
 val binders_offset
-  (c: CH.clientHello {has_binders c})
-: Tot (u: U32.t { U32.v u <= Seq.length (LP.serialize CH.clientHello_serializer c) })
+  (m: H.handshake {has_binders m})
+: Tot (u: U32.t { U32.v u <= Seq.length (LP.serialize H.handshake_serializer m) })
 
 val binders_offset_set_binder
-  (c: CH.clientHello {has_binders c})
-  (b' : Psks.offeredPsks_binders { Psks.offeredPsks_binders_bytesize b' == Psks.offeredPsks_binders_bytesize (get_binders c) } )
+  (m: H.handshake {has_binders m})
+  (b' : Psks.offeredPsks_binders { Psks.offeredPsks_binders_bytesize b' == Psks.offeredPsks_binders_bytesize (get_binders m) } )
 : Lemma
-  (binders_offset (set_binders c b') == binders_offset c)
+  (binders_offset (set_binders m b') == binders_offset m)
 
 module BY = FStar.Bytes
 
 let truncate_clientHello_bytes
-  (c: CH.clientHello {has_binders c})
+  (m: H.handshake {has_binders m})
 : Tot BY.bytes
-= BY.slice (CH.clientHello_serializer32 c) 0ul (binders_offset c)
+= BY.slice (H.handshake_serializer32 m) 0ul (binders_offset m)
 
 val truncate_clientHello_bytes_correct
-  (c: CH.clientHello {has_binders c})
+  (m: H.handshake {has_binders m})
 : Lemma
-  (CH.clientHello_serializer32 c == BY.append (truncate_clientHello_bytes c) (Psks.offeredPsks_binders_serializer32 (get_binders c)))
+  (H.handshake_serializer32 m == BY.append (truncate_clientHello_bytes m) (Psks.offeredPsks_binders_serializer32 (get_binders m)))
 
 val truncate_clientHello_bytes_set_binders
-  (c: CH.clientHello {has_binders c})
-  (b' : Psks.offeredPsks_binders { Psks.offeredPsks_binders_bytesize b' == Psks.offeredPsks_binders_bytesize (get_binders c) } )
+  (m: H.handshake {has_binders m})
+  (b' : Psks.offeredPsks_binders { Psks.offeredPsks_binders_bytesize b' == Psks.offeredPsks_binders_bytesize (get_binders m) } )
 : Lemma
-  (truncate_clientHello_bytes (set_binders c b') == truncate_clientHello_bytes c)
+  (truncate_clientHello_bytes (set_binders m b') == truncate_clientHello_bytes m)
 
 val truncate_clientHello_bytes_inj_binders_bytesize
-  (c1: CH.clientHello {has_binders c1})
-  (c2: CH.clientHello {has_binders c2})
+  (m1: H.handshake {has_binders m1})
+  (m2: H.handshake {has_binders m2})
 : Lemma
-  (requires (truncate_clientHello_bytes c1 == truncate_clientHello_bytes c2))
+  (requires (truncate_clientHello_bytes m1 == truncate_clientHello_bytes m2))
   (ensures (
-    Psks.offeredPsks_binders_bytesize (get_binders c1) == Psks.offeredPsks_binders_bytesize (get_binders c2)
+    Psks.offeredPsks_binders_bytesize (get_binders m1) == Psks.offeredPsks_binders_bytesize (get_binders m2)
   ))
 
 module LPS = LowParse.SLow.Base
 
 let truncate_clientHello_bytes_inj
-  (c1: CH.clientHello {has_binders c1})
-  (c2: CH.clientHello {has_binders c2})
+  (m1: H.handshake {has_binders m1})
+  (m2: H.handshake {has_binders m2})
   (b' : Psks.offeredPsks_binders)
 : Lemma
   (requires (
-    truncate_clientHello_bytes c1 == truncate_clientHello_bytes c2 /\
-    (Psks.offeredPsks_binders_bytesize b' == Psks.offeredPsks_binders_bytesize (get_binders c1) \/ Psks.offeredPsks_binders_bytesize b' == Psks.offeredPsks_binders_bytesize (get_binders c2))
+    truncate_clientHello_bytes m1 == truncate_clientHello_bytes m2 /\
+    (Psks.offeredPsks_binders_bytesize b' == Psks.offeredPsks_binders_bytesize (get_binders m1) \/ Psks.offeredPsks_binders_bytesize b' == Psks.offeredPsks_binders_bytesize (get_binders m2))
   ))
   (ensures (
-    Psks.offeredPsks_binders_bytesize b' == Psks.offeredPsks_binders_bytesize (get_binders c1) /\
-    Psks.offeredPsks_binders_bytesize b' == Psks.offeredPsks_binders_bytesize (get_binders c2) /\
-    set_binders c1 b' == set_binders c2 b'
+    Psks.offeredPsks_binders_bytesize b' == Psks.offeredPsks_binders_bytesize (get_binders m1) /\
+    Psks.offeredPsks_binders_bytesize b' == Psks.offeredPsks_binders_bytesize (get_binders m2) /\
+    set_binders m1 b' == set_binders m2 b'
   ))
-= truncate_clientHello_bytes_inj_binders_bytesize c1 c2;
-  truncate_clientHello_bytes_correct c1;
-  truncate_clientHello_bytes_correct c2;
+= truncate_clientHello_bytes_inj_binders_bytesize m1 m2;
+  truncate_clientHello_bytes_correct m1;
+  truncate_clientHello_bytes_correct m2;
   Psks.offeredPsks_binders_bytesize_eq b';
-  Psks.offeredPsks_binders_bytesize_eq (get_binders c1);
-  Psks.offeredPsks_binders_bytesize_eq (get_binders c2);
-  truncate_clientHello_bytes_correct (set_binders c1 b');
-  truncate_clientHello_bytes_correct (set_binders c2 b');
-  truncate_clientHello_bytes_set_binders c1 b' ;
-  truncate_clientHello_bytes_set_binders c2 b' ;
-  LPS.serializer32_injective _ CH.clientHello_serializer32 (set_binders c1 b') (set_binders c2 b')
+  Psks.offeredPsks_binders_bytesize_eq (get_binders m1);
+  Psks.offeredPsks_binders_bytesize_eq (get_binders m2);
+  truncate_clientHello_bytes_correct (set_binders m1 b');
+  truncate_clientHello_bytes_correct (set_binders m2 b');
+  truncate_clientHello_bytes_set_binders m1 b' ;
+  truncate_clientHello_bytes_set_binders m2 b' ;
+  LPS.serializer32_injective _ H.handshake_serializer32 (set_binders m1 b') (set_binders m2 b')
 
 (* TODO: replace with accessors once we introduce accessors to elements of variable-length lists *)
 
@@ -148,26 +156,26 @@ let valid_truncate_clientHello
   (pos: U32.t)
 : Lemma
   (requires (
-    LP.valid CH.clientHello_parser h sl pos /\
-    has_binders (LP.contents CH.clientHello_parser h sl pos)
+    LP.valid H.handshake_parser h sl pos /\
+    has_binders (LP.contents H.handshake_parser h sl pos)
   ))
   (ensures (
-    let c = LP.contents CH.clientHello_parser h sl pos in
-    let pos' = LP.get_valid_pos CH.clientHello_parser h sl pos in
-    U32.v pos + U32.v (binders_offset c) + Psks.offeredPsks_binders_bytesize (get_binders c) == U32.v pos' /\
-    LP.bytes_of_slice_from_to h sl pos (pos `U32.add` binders_offset c) == BY.reveal (truncate_clientHello_bytes c) /\
-    LP.valid_content_pos Psks.offeredPsks_binders_parser h sl (pos `U32.add` binders_offset c) (get_binders c) pos'
+    let m = LP.contents H.handshake_parser h sl pos in
+    let pos' = LP.get_valid_pos H.handshake_parser h sl pos in
+    U32.v pos + U32.v (binders_offset m) + Psks.offeredPsks_binders_bytesize (get_binders m) == U32.v pos' /\
+    LP.bytes_of_slice_from_to h sl pos (pos `U32.add` binders_offset m) == BY.reveal (truncate_clientHello_bytes m) /\
+    LP.valid_content_pos Psks.offeredPsks_binders_parser h sl (pos `U32.add` binders_offset m) (get_binders m) pos'
   ))
-= let c = LP.contents CH.clientHello_parser h sl pos in
-  LP.serialized_length_eq CH.clientHello_serializer c;
-  truncate_clientHello_bytes_correct c;
-  let b = get_binders c in
+= let m = LP.contents H.handshake_parser h sl pos in
+  LP.serialized_length_eq H.handshake_serializer m;
+  truncate_clientHello_bytes_correct m;
+  let b = get_binders m in
   Psks.offeredPsks_binders_bytesize_eq b;
   LP.serialized_length_eq Psks.offeredPsks_binders_serializer b;
-  LP.valid_valid_exact CH.clientHello_parser h sl pos;
-  let pos' = LP.get_valid_pos CH.clientHello_parser h sl pos in
-  LP.valid_exact_serialize CH.clientHello_serializer h sl pos pos' ;
-  let pos1 = pos `U32.add` binders_offset c in
+  LP.valid_valid_exact H.handshake_parser h sl pos;
+  let pos' = LP.get_valid_pos H.handshake_parser h sl pos in
+  LP.valid_exact_serialize H.handshake_serializer h sl pos pos' ;
+  let pos1 = pos `U32.add` binders_offset m in
   assert (LP.bytes_of_slice_from_to h sl pos1 pos' == Seq.slice (LP.bytes_of_slice_from_to h sl pos pos') (U32.v pos1 - U32.v pos) (U32.v pos' - U32.v pos));
   LP.serialize_valid_exact Psks.offeredPsks_binders_serializer h sl b pos1 pos' ;
   LP.valid_exact_valid Psks.offeredPsks_binders_parser h sl pos1 pos'
@@ -179,23 +187,23 @@ let truncate_clientHello_valid
   (pos: U32.t)
   (pos1: U32.t)
   (pos' : U32.t)
-  (c: CH.clientHello {has_binders c})
+  (m: H.handshake {has_binders m})
 : Lemma
   (requires (
     LP.live_slice h sl /\
     U32.v pos <= U32.v pos1 /\
-    LP.valid_content_pos Psks.offeredPsks_binders_parser h sl pos1 (get_binders c) pos' /\
-    LP.bytes_of_slice_from_to h sl pos pos1 `Seq.equal` BY.reveal (truncate_clientHello_bytes c)
+    LP.valid_content_pos Psks.offeredPsks_binders_parser h sl pos1 (get_binders m) pos' /\
+    LP.bytes_of_slice_from_to h sl pos pos1 `Seq.equal` BY.reveal (truncate_clientHello_bytes m)
   ))
   (ensures (
-    LP.valid_content_pos CH.clientHello_parser h sl pos c pos'
+    LP.valid_content_pos H.handshake_parser h sl pos m pos'
   ))
-= let b = get_binders c in
+= let b = get_binders m in
   LP.valid_valid_exact Psks.offeredPsks_binders_parser h sl pos1 ;
   LP.valid_exact_serialize Psks.offeredPsks_binders_serializer h sl pos1 pos' ;
-  truncate_clientHello_bytes_correct c;
-  LP.serialize_valid_exact CH.clientHello_serializer h sl c pos pos' ;
-  LP.valid_exact_valid CH.clientHello_parser h sl pos pos'
+  truncate_clientHello_bytes_correct m;
+  LP.serialize_valid_exact H.handshake_serializer h sl m pos pos' ;
+  LP.valid_exact_valid H.handshake_parser h sl pos pos'
 
 module B = LowStar.Monotonic.Buffer
 module HST = FStar.HyperStack.ST
@@ -206,15 +214,15 @@ val binders_pos
   (pos: U32.t)
 : HST.Stack U32.t
   (requires (fun h ->
-    LP.valid CH.clientHello_parser h sl pos /\
-    has_binders (LP.contents CH.clientHello_parser h sl pos)
+    LP.valid H.handshake_parser h sl pos /\
+    has_binders (LP.contents H.handshake_parser h sl pos)
   ))
   (ensures (fun h res h' ->
-    let c = LP.contents CH.clientHello_parser h sl pos in
+    let m = LP.contents H.handshake_parser h sl pos in
     B.modifies B.loc_none h h' /\
     U32.v res <= U32.v pos /\
-    U32.v pos + U32.v (binders_offset c) == U32.v res /\
-    LP.valid_content_pos Psks.offeredPsks_binders_parser h sl res (get_binders c) (LP.get_valid_pos CH.clientHello_parser h sl pos)
+    U32.v pos + U32.v (binders_offset m) == U32.v res /\
+    LP.valid_content_pos Psks.offeredPsks_binders_parser h sl res (get_binders m) (LP.get_valid_pos H.handshake_parser h sl pos)
   ))
 
 let valid_binders_mutate
@@ -227,31 +235,31 @@ let valid_binders_mutate
   (h2: HS.mem)
 : Lemma
   (requires (
-    LP.valid CH.clientHello_parser h1 sl pos /\ (
-    let c = LP.contents CH.clientHello_parser h1 sl pos in
-    let pos' = LP.get_valid_pos CH.clientHello_parser h1 sl pos in
-    has_binders c /\
-    U32.v pos + U32.v (binders_offset c) == U32.v pos1 /\
+    LP.valid H.handshake_parser h1 sl pos /\ (
+    let m = LP.contents H.handshake_parser h1 sl pos in
+    let pos' = LP.get_valid_pos H.handshake_parser h1 sl pos in
+    has_binders m /\
+    U32.v pos + U32.v (binders_offset m) == U32.v pos1 /\
     LP.valid_pos Psks.offeredPsks_binders_parser h2 sl pos1 pos' /\
     B.modifies (l `B.loc_union` LP.loc_slice_from_to sl pos1 pos') h1 h2 /\
     B.loc_disjoint l (LP.loc_slice_from_to sl pos pos')
   )))
   (ensures (
-    let c = LP.contents CH.clientHello_parser h1 sl pos in
-    let pos' = LP.get_valid_pos CH.clientHello_parser h1 sl pos in
-    U32.v pos + U32.v (binders_offset c) <= U32.v pos' /\ (
-    let b1 = get_binders c in
+    let m = LP.contents H.handshake_parser h1 sl pos in
+    let pos' = LP.get_valid_pos H.handshake_parser h1 sl pos in
+    U32.v pos + U32.v (binders_offset m) <= U32.v pos' /\ (
+    let b1 = get_binders m in
     let b2 = LP.contents Psks.offeredPsks_binders_parser h2 sl pos1 in
     Psks.offeredPsks_binders_bytesize b1 == Psks.offeredPsks_binders_bytesize b2 /\
-    LP.valid_content_pos CH.clientHello_parser h2 sl pos (set_binders c b2) pos'
+    LP.valid_content_pos H.handshake_parser h2 sl pos (set_binders m b2) pos'
   )))
 = valid_truncate_clientHello h1 sl pos;
-  let pos' = LP.get_valid_pos CH.clientHello_parser h1 sl pos in
-  let c = LP.contents CH.clientHello_parser h1 sl pos in
+  let pos' = LP.get_valid_pos H.handshake_parser h1 sl pos in
+  let m = LP.contents H.handshake_parser h1 sl pos in
   let b2 = LP.contents Psks.offeredPsks_binders_parser h2 sl pos1 in
   LP.content_length_eq Psks.offeredPsks_binders_serializer h2 sl pos1 ;
   LP.serialized_length_eq Psks.offeredPsks_binders_serializer b2;
   Psks.offeredPsks_binders_bytesize_eq b2;
-  truncate_clientHello_bytes_set_binders c b2;
+  truncate_clientHello_bytes_set_binders m b2;
   B.modifies_buffer_from_to_elim sl.LP.base pos pos1 (l `B.loc_union` LP.loc_slice_from_to sl pos1 pos') h1 h2;
-  truncate_clientHello_valid h2 sl pos pos1 pos' (set_binders c b2)
+  truncate_clientHello_valid h2 sl pos pos1 pos' (set_binders m b2)
